src/CircomLib/EdDSA.v
@@ -1,0 +1,211 @@
+Require Import Coq.Lists.List.
+Require Import Coq.micromega.Lia.
+Require Import Coq.Init.Peano.
+Require Import Coq.Arith.PeanoNat.
+Require Import Coq.Arith.Compare_dec.
+Require Import Coq.PArith.BinPosDef.
+Require Import Coq.ZArith.BinInt Coq.ZArith.ZArith Coq.ZArith.Zdiv Coq.ZArith.Znumtheory Coq.NArith.NArith. (* import Zdiv before Znumtheory *)
+Require Import Coq.NArith.Nnat.
+
+Require Import Crypto.Spec.ModularArithmetic.
+Require Import Crypto.Arithmetic.PrimeFieldTheorems Crypto.Algebra.Field.
+Require Import Crypto.Util.Decidable. (* Crypto.Util.Notations. *)
+Require Import Coq.setoid_ring.Ring_theory Coq.setoid_ring.Field_theory Coq.setoid_ring.Field_tac.
+Require Import Ring.
+
+From Circom Require Import Circom Util Default Tuple LibTactics Simplify Repr ListUtil.
+From Circom.CircomLib Require Import Bitify Comparators.
+
+Local Open Scope circom_scope.
+Local Open Scope F_scope.
+Local Open Scope tuple_scope.
+
+Local Notation "x [[ i ]]" := (Tuple.nth_default 0 i x) (at level 20).
+Definition nth2 {m n} (i: nat) (x: (F^n)^m) := Tuple.nth_default (repeat 0 n) i x.
+Local Notation "x [ i ][ j ]" := (Tuple.nth_default 0 j (nth2 i x)) (at level 20).
+Definition nth3 {m n p} (i: nat) (x: ((F^n)^m)^p) := Tuple.nth_default (repeat (repeat 0 n) m) i x.
+Local Notation "x [ i ][ j ][ k ]" := (Tuple.nth_default 0 k (nth2 j (nth3 i x))) (at level 20).
+
+(* Poseidon *)
+Module Poseidon.
+Section Poseidon.
+Context {nInputs: nat}.
+
+Definition cons (inputs: F^nInputs) (out: F) := True.
+
+Record t : Type := 
+{ inputs: F^nInputs;
+  out: F;
+  _cons: cons inputs out; }.
+
+Definition wgen: t. skip. Defined.
+
+#[global] Instance Default: Default t. constructor. exact wgen. Defined.
+
+End Poseidon.
+
+Module PoseidonHypo.
+Axiom poseidon_1 : F -> F.
+Axiom poseidon_2 : F -> F -> F.
+Axiom poseidons_5: F -> F -> F -> F -> F -> F.
+
+Lemma poseidon_1_spec : 
+  forall (p: @Poseidon.t 1) x, p.(inputs)[0] = x -> p.(Poseidon.out) = poseidon_1 x. skip. Defined.
+Lemma poseidon_2_spec :
+  forall (p: @Poseidon.t 2) x y, p.(inputs)[0] = x -> p.(inputs)[1] = y -> p.(Poseidon.out) = poseidon_2 x y. skip. Defined.
+Lemma poseidon_5_spec :
+  forall (p: @Poseidon.t 5) x y z w v, p.(inputs)[0] = x -> p.(inputs)[1] = y -> p.(inputs)[2] = z -> p.(inputs)[3] = w -> p.(inputs)[4] = v -> p.(Poseidon.out) = poseidons_5 x y z w v. skip. Defined.
+
+End PoseidonHypo.
+
+End Poseidon.
+
+
+
+(* Source: https://github.com/iden3/circomlib/blob/master/circuits/eddsaposeidon.circom *)
+Module EdDSAPoseidonVerifier.
+Module Poseidon:= Poseidon.
+Module Cmp := Comparators.
+Import Cmp.
+Section EdDSAPoseidonVerifier.
+
+Definition poseidons_5 := Poseidon.PoseidonHypo.poseidons_5.
+
+Axiom BabyDbl: F -> F -> F*F.
+
+Axiom edwards_mult: F -> F -> F -> F*F.
+
+Axiom edwards_add: F -> F -> F -> F -> F*F.
+
+Definition q1 := (F.of_nat q 5299619240641551281634865583518297030282874472190772894086521144482721001553).
+Definition q2 := (F.of_nat q 16950150798460657717958625567821834550301663161624707787222815936182638968203).
+
+Definition eddsa_poseidon Ax Ay S R8x R8y M := 
+  let hash := poseidons_5 R8x R8y Ax Ay M in
+  let '(dbl1_xout, dbl1_yout)  := BabyDbl Ax Ay in
+  let '(dbl2_xout, dbl2_yout)  := BabyDbl dbl1_xout dbl1_yout in
+  let '(dbl3_xout, dbl3_yout)  := BabyDbl dbl2_xout dbl2_yout in
+  let '(right2_x, right2_y)  := edwards_mult hash dbl3_xout dbl3_yout in
+  let '(right_x, right_y) := edwards_add R8x R8y right2_x right2_y in
+  let '(left_x, left_y) := edwards_mult S q1 q2 in
+  left_x = right_x /\ left_y = right_y.
+
+Definition cons (enabled: F) (Ax: F) (Ay: F) (S: F) (R8x: F) (R8y: F) (M: F) :=
+  exists (hash: @Poseidon.t 5) (eqCheckX eqCheckY: ForceEqualIfEnabled.t), 
+    (hash.(Poseidon.inputs)[0] = R8x) /\
+    (hash.(Poseidon.inputs)[1] = R8y) /\
+    (hash.(Poseidon.inputs)[2] = Ax) /\
+    (hash.(Poseidon.inputs)[3] = Ay) /\
+    (hash.(Poseidon.inputs)[4] = M) /\
+    let '(dbl1_xout, dbl1_yout)  := BabyDbl Ax Ay in
+    let '(dbl2_xout, dbl2_yout)  := BabyDbl dbl1_xout dbl1_yout in
+    let '(dbl3_xout, dbl3_yout)  := BabyDbl dbl2_xout dbl2_yout in
+    let '(right2_x, right2_y)  := edwards_mult hash.(Poseidon.out) dbl3_xout dbl3_yout in
+    let '(right_x, right_y) := edwards_add R8x R8y right2_x right2_y in
+    let '(left_x, left_y) := edwards_mult S q1 q2 in
+    eqCheckX.(ForceEqualIfEnabled.enabled) = enabled /\
+    eqCheckX.(ForceEqualIfEnabled._in)[0] = left_x /\
+    eqCheckX.(ForceEqualIfEnabled._in)[1] = right_x /\
+    eqCheckY.(ForceEqualIfEnabled.enabled) = enabled /\
+    eqCheckY.(ForceEqualIfEnabled._in)[0] = left_y /\
+    eqCheckY.(ForceEqualIfEnabled._in)[1] = right_y.
+
+Record t : Type := 
+{ enabled: F;
+  Ax: F;
+  Ay: F;
+  S: F;
+  R8x: F;
+  R8y: F;
+  M: F;
+  _cons: cons enabled Ax Ay S R8x R8y M; }.
+
+Definition wgen: t. skip. Defined.
+
+#[global] Instance Default: Default t. constructor. exact wgen. Defined.
+
+End EdDSAPoseidonVerifier.
+
+Module EdDSAPoseidonVerifierProof.
+
+Lemma EdDSAPoseidonVerifier_spec :
+  forall (p: @EdDSAPoseidonVerifier.t),
+    p.(enabled) <> 0 ->
+    eddsa_poseidon p.(Ax) p.(Ay) p.(S) p.(R8x) p.(R8y) p.(M).
+Proof.
+  intros. unwrap_C. destruct p eqn:hh;simpl in *.
+  unfold cons in *.
+  destruct _cons0. simpl in *. destruct p;simpl in *.
+  destruct e.
+  destruct e. pose proof a.
+  intuition. 
+  destruct BabyDbl eqn: db1 in H6.
+  destruct BabyDbl eqn: db2 in H6.
+  destruct BabyDbl eqn: db3 in H6.
+  destruct edwards_mult eqn: em in H6.
+  destruct edwards_add eqn: ea in H6.
+  destruct edwards_mult eqn: em2 in H6.
+  intuition.
+  subst.
+  unfold eddsa_poseidon.
+  rewrite db1, db2, db3.
+  erewrite <- (Poseidon.PoseidonHypo.poseidon_5_spec x);eauto.
+  rewrite em, ea, em2.
+  pose proof (Cmp.ForceEqualIfEnabled.soundness x0). 
+  pose proof (Cmp.ForceEqualIfEnabled.soundness x1).
+  simpl in *. subst. intuit.
+  apply H1;auto. rewrite H8. auto.
+Qed.
+
+Definition unconstrained:= ForceEqualIfEnabled.unconstrained.
+
+(* forall Ax Ay S R8x R8y M, EdDSAPoseidonVerifier 0 Ax Ay S R8x R8y M *)
+Lemma EdDSAPoseidonVerifier_spec_disabled :
+  forall Ax Ay S R8x R8y M (hash: @Poseidon.t 5) (eqCheckX eqCheckY: ForceEqualIfEnabled.t),
+    (hash.(Poseidon.inputs)[0] = R8x) ->
+    (hash.(Poseidon.inputs)[1] = R8y) ->
+    (hash.(Poseidon.inputs)[2] = Ax) ->
+    (hash.(Poseidon.inputs)[3] = Ay) ->
+    (hash.(Poseidon.inputs)[4] = M) ->
+    let
+    '(dbl1_xout, dbl1_yout) := BabyDbl Ax Ay in
+     let
+     '(dbl2_xout, dbl2_yout) := BabyDbl dbl1_xout dbl1_yout
+      in
+      let
+      '(dbl3_xout, dbl3_yout) := BabyDbl dbl2_xout dbl2_yout
+       in
+       let
+       '(right2_x, right2_y) :=
+        edwards_mult (Poseidon.out hash) dbl3_xout dbl3_yout
+        in
+        let
+        '(right_x, right_y) :=
+         edwards_add R8x R8y right2_x right2_y in
+         let
+         '(left_x, left_y) := edwards_mult S q1 q2 in
+    eqCheckX.(ForceEqualIfEnabled.enabled) = 0 /\
+    eqCheckX.(ForceEqualIfEnabled._in)[0] = left_x /\
+    eqCheckX.(ForceEqualIfEnabled._in)[1] = right_x /\
+    eqCheckY.(ForceEqualIfEnabled.enabled) = 0 /\
+    eqCheckY.(ForceEqualIfEnabled._in)[0] = left_y /\
+    eqCheckY.(ForceEqualIfEnabled._in)[1] = right_y ->
+    unconstrained left_x right_x /\ unconstrained left_y right_y.
+Proof.
+  intros.
+  destruct BabyDbl eqn: db1.
+  destruct (BabyDbl f _) eqn: db2.
+  destruct (BabyDbl f1 _) eqn: db3.
+  destruct edwards_mult eqn: em.
+  destruct edwards_add eqn: ea.
+  destruct (edwards_mult S0 _ _) eqn: em2. subst. 
+  intuit.
+  pose proof (Cmp.ForceEqualIfEnabled.circuit_disabled eqCheckX);intuit.
+  rewrite <-H1,<-H. unfold unconstrained. auto.
+  pose proof (Cmp.ForceEqualIfEnabled.circuit_disabled eqCheckY);intuit.
+  rewrite <-H3,<-H5. unfold unconstrained. auto. 
+Qed.
+
+End EdDSAPoseidonVerifierProof.
+
+End EdDSAPoseidonVerifier.
